Completed merge and share for permissionned arrays Added an init_ghost to FStar.Seq LowStar.Permissions is now all-Tot instead of GTot

ulib/LowStar.Permissions.Array.fsti
@@ -3,6 +3,8 @@ module LowStar.Permissions.Array
 module HS = FStar.HyperStack
 open FStar.HyperStack.ST
 module U32 = FStar.UInt32
+module PR = LowStar.Permissions.References
+module P = LowStar.Permissions
 
 val array (a:Type0): Type0
 
@@ -10,19 +12,45 @@ val array (a:Type0): Type0
 
 val length (#a:Type) (b:array a) : nat
 
-val live (#a:Type) (h:HS.mem) (b:array a) : Type0
-val writeable (#a:Type) (h:HS.mem) (b:array a) : Type0
-
-val lemma_writeable_implies_live (#a:Type) (h:HS.mem) (b:array a)
-  : Lemma (requires writeable h b)
-          (ensures live h b)
-
 val as_seq (#a:Type) (h:HS.mem) (b:array a) : GTot (s:Seq.seq a{Seq.length s == length b})
+
+val as_perm_seq (#a:Type) (h:HS.mem) (b:array a) : GTot (s:Seq.seq P.permission{Seq.length s == length b})
 
 let get (#a:Type) (h:HS.mem) (b:array a) (i:nat{i < length b}) : GTot a
   = Seq.index (as_seq h b) i
 
+let get_perm (#a:Type) (h:HS.mem) (b:array a) (i:nat{i < length b}) : GTot P.permission
+  = Seq.index (as_perm_seq h b) i
+
+
+val live (#a:Type) (h:HS.mem) (b:array a) : Type0
+
+let writeable_cell (#a:Type) (h:HS.mem) (b:array a) (i:nat{i < length b}) : Type0 =
+  get_perm #a h b i == 1.0R /\ live #a h b
+
+let writeable #a h b =
+  live #a h b /\
+  (forall (i:nat{i < length #a b}). writeable_cell h b i)
+
+
 val mergeable (#a:Type0) (b1 b2:array a) : Type0
+
+val mergeable_same_length (#a:Type0) (b1 b2:array a) : Lemma
+  (requires (mergeable b1 b2))
+  (ensures (length b1 = length b2))
+  [SMTPatOr [
+    [SMTPat (mergeable b1 b2); SMTPat (length b1)];
+    [SMTPat (mergeable b1 b2); SMTPat (length b2)]
+  ]]
+
+val mergeable_comm (#a: Type0) (b1 b2: array a): Lemma
+  (requires (mergeable b1 b2))
+  (ensures (mergeable b2 b1))
+  [SMTPat (mergeable b1 b2)]
+
+let summable_permissions (#a: Type0) (h: HS.mem) (b1 b2: array a) : Type0 =
+  mergeable #a b1 b2 /\
+  (forall (i:nat{i < length #a b1}). P.summable_permissions (get_perm h b1 i) (get_perm h b2 i))
 
 val frameOf (#a:Type0) (b:array a) : Tot HS.rid
 val as_addr (#a:Type0) (b:array a) : GTot nat
@@ -48,8 +76,8 @@ val index (#a:Type) (b:array a) (i:U32.t{U32.v i < length b})
             (ensures fun h0 y h1 -> h0 == h1 /\ y == get h0 b (U32.v i))
 
 val upd (#a:Type) (b:array a) (i:U32.t{U32.v i < length b}) (v:a)
-    : Stack unit (requires fun h -> writeable h b)
-                 (ensures fun h0 _ h1 ->  writeable h1 b /\
+    : Stack unit (requires fun h -> writeable_cell h b (U32.v i))
+                 (ensures fun h0 _ h1 ->  writeable_cell h1 b (U32.v i) /\
                                        modifies (loc_array b) h0 h1 /\
                                        as_seq h1 b == Seq.upd (as_seq h0 b) (U32.v i) v)
 
@@ -70,18 +98,38 @@ val sub (#a:Type) (b:array a) (i:U32.t) (len:U32.t)
 val alloc (#a:Type0) (init:a) (len:U32.t)
   : ST (array a)
        (requires fun _ -> U32.v len > 0)
-       (ensures fun h0 b h1 -> 
-         modifies loc_none h0 h1 /\ 
-         writeable h1 b /\ 
+       (ensures fun h0 b h1 ->
+         modifies loc_none h0 h1 /\
+         writeable h1 b /\
          as_seq h1 b == Seq.create (U32.v len) init)
 
 val share (#a:Type0) (b:array a) : Stack (array a)
   (requires fun h0 -> live h0 b /\ length b > 0)
-  (ensures fun h0 b' h1 -> 
-    modifies (loc_array b) h0 h1 /\ 
+  (ensures fun h0 b' h1 ->
+    modifies (loc_array b) h0 h1 /\
     live h1 b /\ live h1 b' /\
     loc_disjoint (loc_array b) (loc_array b') /\
     as_seq h0 b == as_seq h1 b /\ // The values of the initial array are not modified
-    as_seq h1 b' == as_seq h1 b /\ // The values of the new buffer are the same as the initial array
+    as_seq h1 b' == as_seq h1 b /\ // The values of the new array are the same as the initial array
     mergeable b b' /\
-    True) // TODO: Talk about permissions here?
+    (forall (i:nat{i < length b}). {:pattern [get_perm h1 b' i; get_perm h1 b i] } // The permission gets split in two
+      get_perm h1 b' i == P.half_permission (get_perm h0 b i) /\
+      get_perm h1 b i == P.half_permission (get_perm h0 b i)
+    ))
+
+val merge:
+  #a: Type ->
+  b: array a ->
+  b1: array a ->
+  Stack unit (requires (fun h0 ->
+    mergeable b b1 /\
+    live h0 b /\ live h0 b1 /\
+    (forall (i:nat{i < length b}). summable_permissions h0 b b1  )
+  ))
+  (ensures (fun h0 _ h1 ->
+    live h1 b /\ (forall (i:nat{i < length b}). {:pattern (get_perm h1 b i)} // Permissions are summed into the first array
+      get_perm h1 b i =  P.sum_permissions (get_perm h0 b i) (get_perm h0 b1 i)
+    ) /\
+    as_seq h1 b == as_seq h0 b /\ // The value of the array are not modifies
+    modifies (loc_array b `loc_union` loc_array b1) h0 h1
+  ))
